Pushed branch updated version of hw2a

hw2a-dafny-tutorial-brighamband/tcp.dfy
@@ -16,15 +16,32 @@ class ClientTcpConnection {
 
   var state: STATE
 
+   /**
+   * Constructor: state will always start as CLOSED
+   */
+  constructor init()
+    ensures state == CLOSED
+  {
+    state := CLOSED;
+  }
+
   // Helper methods
   method sendSyn()  
+    modifies `state
+    ensures state == SYN_SENT
   {
-    // TODO
+    state := SYN_SENT;
   }
 
   method recvSynAck()
+    modifies `state
+    ensures old(state) == SYN_SENT ==> state == ESTABLISHED
+    ensures old(state) != SYN_SENT ==> state == old(state)
   {
-    // TODO
+    if (state == SYN_SENT)
+    {
+      state := ESTABLISHED;
+    }
   }
 
   /**
@@ -36,25 +53,188 @@ class ClientTcpConnection {
   }
 
   method sendFin()
+    modifies `state
+    ensures old(state) == CLOSE_WAIT ==> state == LAST_ACK
+    ensures old(state) != CLOSE_WAIT ==> state == FIN_WAIT_1
   {
-    // TODO
+    if (state == CLOSE_WAIT)
+    {
+      state := LAST_ACK;
+    }
+    else 
+    {
+      state := FIN_WAIT_1;
+    }
   }
 
   method recvAck()
+    modifies `state
+    ensures old(state) == FIN_WAIT_1 ==> state == FIN_WAIT_2
+    ensures old(state) == LAST_ACK ==> state == CLOSED
   {
-    // TODO
+    if (state == FIN_WAIT_1)
+    {
+      state := FIN_WAIT_2;
+    }
+    else if (state == LAST_ACK)
+    {
+      state := CLOSED;
+    }
   }
 
   method recvFin()
+    modifies `state
+    ensures old(state) == FIN_WAIT_2 ==> state == TIME_WAIT
+    ensures old(state) != FIN_WAIT_2 ==> state == CLOSE_WAIT
   {
-    // TODO
+    if (state == FIN_WAIT_2)
+    {
+      state := TIME_WAIT;
+    }
+    else
+    {
+      state := CLOSE_WAIT;
+    }
   }
 
   method timeout()
+    modifies `state
+    ensures state == CLOSED
   {
-    // TODO
+    state := CLOSED;
   }
 
-  // TODO: Add code from tutorial here.
+  method isClosed() returns (result: bool)
+    ensures result == (state == CLOSED)
+  {
+    if (state == CLOSED)
+    {
+      result := true;
+    }
+    else 
+    {
+      result := false;
+    }
+  }
 
+  method isEstablished() returns (result: bool)
+    ensures result == (state == ESTABLISHED)
+  {
+    if (state == ESTABLISHED)
+    {
+      result := true;
+    }
+    else 
+    {
+      result := false;
+    }
+  }
+
+  /**
+  * This method represents a client starting the 3-way handshake
+  *   with a server to establish a TCP connection.
+  */
+  method connect()
+    modifies `state
+    ensures old(state) == CLOSED ==> state == ESTABLISHED
+    ensures old(state) != CLOSED ==> state == old(state)
+  {
+    if (state == CLOSED)
+    {
+      sendSyn();
+      recvSynAck();
+      sendAck();
+    }
+  }
+
+  /**
+  * This method represents a client starting the 4-way handshake
+  *   with a server to close an established TCP connection.
+  */
+  method close()
+    modifies `state
+    ensures state == CLOSED
+  {
+    if (state != CLOSED)
+    {
+      sendFin();
+      recvAck();
+      recvFin();
+      sendAck();
+      timeout();
+    }
+  }
+
+  /**
+  * This method represents a client terminating an established
+  *   TCP connection from a server request to close.
+  */
+  method terminate()
+    modifies `state
+    requires state == ESTABLISHED
+    ensures state == CLOSED
+  {
+    recvFin();
+    sendAck();
+    sendFin();
+    recvAck();
+  }
+
+  /**
+  * Test client initiate connect
+  */
+  method test_ClientConnect()
+  {
+    var client := new ClientTcpConnection.init();
+    var isClosed: bool := client.isClosed();
+    assert (isClosed);
+    client.connect();
+    var isEstablished: bool := client.isEstablished();
+    assert (isEstablished);
+  }
+
+  /**
+  * Test client initiate close after connect
+  */
+  method test_ClientConnectThenClientClose()
+  {
+    var client := new ClientTcpConnection.init();
+    var isClosed: bool := client.isClosed();
+    assert (isClosed);
+    client.connect();
+    var isEstablished: bool := client.isEstablished();
+    assert (isEstablished);
+    client.close();
+    isClosed := client.isClosed();
+    assert (isClosed);
+  }
+
+  /**
+  * Test server initiate close after connect
+  */
+  method test_ClientConnectThenServerClose()
+  {
+    var client := new ClientTcpConnection.init();
+    var isClosed: bool := client.isClosed();
+    assert (isClosed);
+    client.connect();
+    var isEstablished: bool := client.isEstablished();
+    assert (isEstablished);
+    client.terminate();
+    isClosed := client.isClosed();
+    assert (isClosed);
+  }
+
+  /**
+  * Test calling 'close' twice
+  */
+  method test_ClientCloseTwice()
+  {
+    var client := new ClientTcpConnection.init();
+    var isClosed: bool := client.isClosed();
+    assert (isClosed);
+    client.close();
+    isClosed := client.isClosed();
+    assert (isClosed);
+  }
 }
